### Matrix Multiplication of \( A \) and \( B \)

We are given:

\[
A = \begin{bmatrix}
-1 & 2 & 3 \\
4 & -5 & 6 \\
7 & 8 & -9
\end{bmatrix}, \quad
B = \begin{bmatrix}
0 & 2 & 1 \\
0 & 2 & -8 \\
2 & 9 & -1
\end{bmatrix}
\]

The product \( C = A \times B \) is calculated by taking the dot product of each row of \( A \) with each column of \( B \). The resulting matrix \( C \) will also be \( 3 \times 3 \).

---

### General Formula

The element \( c_{ij} \) of \( C \) is given by:
\[
c_{ij} = \sum_{k=1}^{n} a_{ik} \cdot b_{kj}
\]
Where:
- \( a_{ik} \) is the element from the \( i \)-th row of \( A \),
- \( b_{kj} \) is the element from the \( j \)-th column of \( B \).

---

### Step-by-Step Calculation

#### 1. First Row of \( C \)
- **Element \( c_{11} \):**
  \[
  c_{11} = (-1)(0) + (2)(0) + (3)(2) = 0 + 0 + 6 = 6
  \]

- **Element \( c_{12} \):**
  \[
  c_{12} = (-1)(2) + (2)(2) + (3)(9) = -2 + 4 + 27 = 29
  \]

- **Element \( c_{13} \):**
  \[
  c_{13} = (-1)(1) + (2)(-8) + (3)(-1) = -1 - 16 - 3 = -20
  \]

#### 2. Second Row of \( C \)
- **Element \( c_{21} \):**
  \[
  c_{21} = (4)(0) + (-5)(0) + (6)(2) = 0 + 0 + 12 = 12
  \]

- **Element \( c_{22} \):**
  \[
  c_{22} = (4)(2) + (-5)(2) + (6)(9) = 8 - 10 + 54 = 52
  \]

- **Element \( c_{23} \):**
  \[
  c_{23} = (4)(1) + (-5)(-8) + (6)(-1) = 4 + 40 - 6 = 38
  \]

#### 3. Third Row of \( C \)
- **Element \( c_{31} \):**
  \[
  c_{31} = (7)(0) + (8)(0) + (-9)(2) = 0 + 0 - 18 = -18
  \]

- **Element \( c_{32} \):**
  \[
  c_{32} = (7)(2) + (8)(2) + (-9)(9) = 14 + 16 - 81 = -51
  \]

- **Element \( c_{33} \):**
  \[
  c_{33} = (7)(1) + (8)(-8) + (-9)(-1) = 7 - 64 + 9 = -48
  \]

---

### Final Matrix

\[
C = \begin{bmatrix}
6 & 29 & -20 \\
12 & 52 & 38 \\
-18 & -51 & -48
\end{bmatrix}
\]
